Track slice capacity
Track slice capacity with appropriate non-deterministic extra allocation
(including at `make` time since the translator allows but ignores any
extra capacity argument). I believe this faithfully models Go's intended
semantics, although the specification is rather vague about how
capacities are updated.

Note that this fixes the unsoundness from not having deallocation in
SliceAppend and removes the need to have deallocation at all.

This complicates proofs in a subtle way: we now have a "large" is_slice
that includes points-to facts for the extra capacity and a "small"
is_slice_small that only has the slice's values. It turns out that
is_slice_small is what you want in most cases because it's a weaker
assumption - it doesn't require the caller to precisely track capacity,
which is what most code does.

The annoying thing is that now sometimes you have to weaken is_slice,
which just adds annoying work because the generic theorems need to be as
strong as possible.

We can fix all of this with the right slice library and probably need to
start putting a layer of abstraction so it's easier to use the slice
library in different ways and have the proofs nicely layered (right now
callers often unfold is_slice, which is bad for making deep changes).

src/program_proof/marshal_proof.v
@@ -198,7 +198,7 @@ Definition is_enc (enc: EncM.t) (vs: Rec): iProp Σ :=
   let encoded := encode vs in
   let encoded_len := Z.of_nat (length encoded) in
   enc.(EncM.off) ↦ (Free #(U64 encoded_len)) ∗
-  enc.(EncM.s).(Slice.ptr) ↦∗[byteT] fmap b2val encoded ∗
+  enc.(EncM.s).(Slice.ptr) ↦∗[byteT] (b2val <$> encoded) ∗
   ∃ (free: list u8),
     (enc.(EncM.s).(Slice.ptr) +ₗ encoded_len) ↦∗[byteT] fmap b2val free ∗
     ⌜(length encoded + length free)%nat = int.nat (EncSz enc)⌝.
@@ -213,11 +213,10 @@ Proof using Type.
   rewrite /struct.buildStruct /Enc.S /=.
   wp_call.
   wp_apply wp_new_slice.
-  iIntros (sl) "[Ha %]".
+  iIntros (sl) "Hs". iDestruct (is_slice_elim with "Hs") as "[Ha %]".
   rewrite replicate_length in H.
   change (int.nat 4096) with (Z.to_nat 4096) in H.
   wp_apply wp_alloc; auto.
-  { repeat econstructor. }
   iIntros (l) "(Hl&_)".
   wp_steps.
   rewrite EncM.to_val_intro.
@@ -252,7 +251,7 @@ Proof using Type.
   { iPureIntro.
     len. }
   wp_apply (wp_UInt64Put with "[Hfree]").
-  { rewrite /is_slice /=.
+  { rewrite /is_slice_small /=.
     iSplitL; [ iSplitL | ].
     - iFramePtsTo by word.
     - len.
@@ -313,7 +312,7 @@ Proof.
 Qed.
 
 Theorem wp_Enc__PutInts stk E enc vs (s:Slice.t) (xs: list u64) :
-  {{{ is_enc enc vs ∗ is_slice s uint64T (u64val <$> xs) ∗
+  {{{ is_enc enc vs ∗ is_slice_small s uint64T (u64val <$> xs) ∗
              ⌜length (encode vs) + 8 * length xs <= int.val (EncSz enc)⌝ }}}
     Enc__PutInts (EncM.to_val enc) (slice_val s) @ stk; E
   {{{ RET #(); is_enc enc (vs ++ (EncUInt64 <$> xs)) }}}.
@@ -343,7 +342,7 @@ Proof using Type.
   - rewrite take_0 app_nil_r.
     iFrame.
   - iIntros "(Henc&Hs)"; iApply "HΦ".
-    iDestruct (is_slice_sz with "Hs") as %Hslen.
+    iDestruct (is_slice_small_sz with "Hs") as %Hslen.
     rewrite fmap_length in Hslen.
     rewrite -> take_ge by lia.
     iFrame.
@@ -366,7 +365,7 @@ Proof using Type.
   { iPureIntro.
     len. }
   wp_apply (wp_UInt32Put with "[Hfree]").
-  { rewrite /is_slice /=.
+  { rewrite /is_slice_small /=.
     iSplitL; [ iSplitL | ].
     - iFramePtsTo by word.
     - len.
@@ -471,7 +470,7 @@ Theorem wp_Enc__Finish stk E enc vs :
   {{{ is_enc enc vs }}}
     Enc__Finish (EncM.to_val enc) @ stk; E
   {{{ s (extra: list u8), RET (slice_val s);
-      is_slice s byteT (b2val <$> encode vs ++ extra) ∗
+      is_slice_small s byteT (b2val <$> encode vs ++ extra) ∗
       ⌜Slice.sz s = EncSz enc⌝ }}}.
 Proof using Type.
   iIntros (Φ) "Henc HΦ".
@@ -507,7 +506,7 @@ Definition is_dec (dec: DecM.t) vs: iProp Σ :=
   ⌜(int.val off + length encoded + Z.of_nat (length extra))%Z = int.val (DecSz dec)⌝.
 
 Theorem wp_NewDec stk E s vs (extra: list u8) :
-  {{{ is_slice s byteT (b2val <$> encode vs ++ extra) }}}
+  {{{ is_slice_small s byteT (b2val <$> encode vs ++ extra) }}}
     NewDec (slice_val s) @ stk; E
   {{{ dec, RET (DecM.to_val dec); is_dec dec vs ∗ ⌜DecSz dec = s.(Slice.sz)⌝ }}}.
 Proof using Type.
@@ -663,13 +662,11 @@ Proof using Type.
   rewrite /Dec__GetInts.
   iIntros (Φ) "(Hdec&%) HΦ".
   wp_pures.
-  wp_apply wp_alloc; auto.
-  { apply zero_val_ty'. }
+  wp_apply (wp_alloc _ _ (slice.T uint64T)); auto.
   iIntros (l) "Hl".
   rewrite zero_slice_val.
   wp_pures.
   wp_apply wp_alloc; auto.
-  { repeat constructor. }
   iIntros (l__i) "Hli".
   wp_let.
   wp_apply (wp_forUpto (λ x,
@@ -717,7 +714,7 @@ Proof using Type.
     iFrame.
     iDestruct (u64_ptsto_untype with "Hli") as "Hli".
     iFrame.
-    iExists (Slice.mk null (U64 0)); iFrame.
+    iExists (Slice.mk null (U64 0) (U64 0)); iFrame.
     rewrite take_0 fmap_nil.
     iApply is_slice_zero.
   - iIntros "[(Hdec&Hslice) Hli]".
